WIP proofs.

src/Oml/MWE4.lean
@@ -1,4 +1,3 @@
-
 import Lean.Data.HashMap
 import Lean.Data.HashSet
 namespace MWE4
@@ -7,8 +6,7 @@ structure State where
   declarations: Lean.HashMap String (Lean.HashSet String)
 
 -- all declaration values must be declaration keys
-def State.wff: State → Bool :=
-  fun s => s.declarations.toList.all fun (_, xs) => xs.toList.all s.declarations.contains
+def State.wff: State → Bool := fun s => s.declarations.toList.all fun (_, xs) => xs.toList.all s.declarations.contains
 
 def State.withDeclaration (s: State) (d: String) : State := 
   match s.declarations.contains d with
@@ -19,12 +17,8 @@ def State.withSpecialization (s: State) (sub: String) (sup: String): State :=
   let s := s.withDeclaration sup
   { s with declarations := s.declarations.insert sub ((s.declarations.findD sub .empty).insert sup) }
 
-theorem State.withDeclarationWff (s: State) (d: String) : s.wff = true → (s.withDeclaration d).wff = true := by
-  intro h
-  sorry
+theorem State.withDeclarationWff (s: State) (d: String) : s.wff → (s.withDeclaration d).wff := sorry
 
-theorem State.withSpecializationWff (s: State) (sub: String) (sup: String): s.wff = true → (s.withSpecialization sub sup).wff = true := by
-  intro h
-  sorry
+theorem State.withSpecializationWff (s: State) (sub: String) (sup: String): s.wff → (s.withSpecialization sub sup).wff := sorry
 
 end MWE4
