src/Oml/MWE5.lean
@@ -2,35 +2,98 @@ import Std.Data.AssocList
 
 namespace MWE5
 
-abbrev Sups := Std.AssocList String Unit
+abbrev Strings := List String
+abbrev Sups := Std.AssocList String Strings
+instance : Repr Sups where reprPrec s n := s.toList.repr n
 
 structure State where
-  declarations: Std.AssocList String Sups
+  declarations: Std.AssocList String Strings := .nil
+  deriving Repr
+
+def State.empty: State := {}
 
 -- all declaration values must be declaration keys
-def State.wff: State → Prop :=
+def State.wff: State → Bool :=
   fun s => s.declarations.all 
     fun (_ sups) => sups.all 
-      fun (sup _) => s.declarations.contains sup
+      fun sup => s.declarations.contains sup
 
 def State.withDeclaration (s: State) (d: String) : State := 
   match s.declarations.contains d with
   | true => s
-  | false => { s with declarations := s.declarations.replace d .nil }
+  | false => { s with declarations := s.declarations.cons d .nil }
 
 def State.withSpecialization (s: State) (sub: String) (sup: String): State :=
-  let s := s.withDeclaration sup
-  let sups : Sups := match s.declarations.find? sub with 
-  | none => .nil
-  | some x => x.replace sup ()
+  let s := s.withDeclaration sub |>.withDeclaration sup
+  let sups : Strings := match s.declarations.find? sub with 
+  | none => 
+    -- this case can never happen since sub has been declared.
+    [sup]
+  | some xs => 
+    if xs.contains sup then xs else xs.cons sup
   { s with declarations := s.declarations.replace sub sups }
 
-theorem State.withDeclarationWff (s: State) (d: String) : s.wff → (s.withDeclaration d).wff := by
+theorem State.withDeclaration.noChange (s: State) (d: String) (h: s.declarations.contains d) 
+: s = s.withDeclaration d 
+:= by rw [State.withDeclaration, h]
+
+theorem State.withDeclaration.added1 (s: State) (d: String) (h: !s.declarations.contains d) 
+: (s.withDeclaration d).declarations.contains d
+:= by 
+  rw [State.withDeclaration] at *
+  simp_all
+
+theorem State.withDeclaration.added2 (s: State) (d: String) (h: !s.declarations.contains d) 
+: (s.withDeclaration d).declarations.find? d = some []
+:= by 
+  rw [State.withDeclaration] at *
+  simp_all
+
+theorem State.withDeclaration.wff (s: State) (d: String) 
+: s.wff → (s.withDeclaration d).wff 
+:= by 
+  simp_all [State.wff, State.withDeclaration]
   intro h
+  split
+  . apply h
+  . simp_all
+    
+    sorry
+    
+    
+theorem State.withSpecialization.noChange (s: State) (sub: String) (sup: String)
+(h1: s.declarations.contains sub) 
+(h2: s.declarations.contains sup) 
+(h3: (s.declarations.find? sub).all (fun sups => sups.contains sup))
+: s = s.withSpecialization sub sup
+:= by
+  --unfold State.withSpecialization State.withDeclaration at *
+  simp [State.withSpecialization, State.withDeclaration] at *
+  simp_all
+  apply h3
   sorry
 
-theorem State.withSpecializationWff (s: State) (sub: String) (sup: String): s.wff → (s.withSpecialization sub sup).wff := by
-  intro h
+theorem State.withSpecialization.added (s: State) (sub: String) (sup: String)
+(h1: !s.declarations.contains sub) 
+(h2: !s.declarations.contains sup) 
+: (s.withSpecialization sub sup).declarations.contains sub && 
+  (s.withSpecialization sub sup).declarations.contains sup
+:= by
+  rw [State.withSpecialization] at *
+  simp [State.withDeclaration, Std.AssocList.contains, List.any, List.replaceF] at *
+  simp_all
+  apply And.intro
   sorry
+
+theorem State.withSpecialization.wff (s: State) (sub: String) (sup: String)
+: s.wff → (s.withSpecialization sub sup).wff 
+:= by
+  simp [State.wff, State.withSpecialization, State.withDeclaration] at *
+  intro h
+  simp [*] at *
+  sorry
+
+def s0 : State := State.empty |>.withSpecialization "a" "b"
+#eval s0
 
 end MWE5
