src/Oml/MWE6.lean
@@ -1,0 +1,74 @@
+import Std.Data.AssocList
+
+namespace MWE6
+
+inductive Syntax where
+  | leaf
+  | withDeclaration (d: String) (s: Syntax) 
+  | withSpecialization (sub: String) (sup: String) (s: Syntax)
+  deriving Repr
+
+def s1 := Syntax.leaf |>.withDeclaration "a" |>.withSpecialization "a" "b"
+#eval s1
+
+abbrev Strings := List String
+
+abbrev Sups := Std.AssocList String Strings
+instance : Repr Sups where reprPrec s n := s.toList.repr n
+
+structure State where
+  decls: Strings := .nil
+  specializations: Sups := .nil
+  deriving Repr
+
+def State.wff(s: State) : Prop :=
+  s.specializations.all 
+    fun (sub sups) => 
+      s.decls.contains sub &&
+      sups.all (fun sup => s.decls.contains sup)
+
+def State.empty: State := {}
+
+theorem State.empty.wff : State.empty.wff := by rfl
+
+def State.withDecl (s: State) (d: String) : State :=
+  match s.decls.contains d with
+  | true    => s
+  | false   => { s with decls := d :: s.decls }
+
+
+theorem State.withDecl.noChange (s: State) (d: String) (h: s.decls.contains d) : s = s.withDecl d := by {
+  sorry
+}
+
+theorem State.withDecl.added (s: State) (d: String) (h: ! s.decls.contains d) : (s.withDecl d).decls.contains d := by {
+  sorry
+}
+
+theorem State.withDecl.wff (s: State) (d: String) (h: s.wff) : s.withDecl d |>.wff := by {
+  sorry
+}
+
+-- To ensure WFF, make sure sub and sup are declared.
+def State.withSpecialization (s: State) (sub: String) (sup: String) : State :=
+  let s' := s.withDecl sub |>.withDecl sup
+  let sups : Strings := match s'.specializations.find? sub with 
+    | none => [sup]
+    | some xs => if xs.contains sup then xs else xs.cons sup
+  match s'.specializations.contains sub with
+  | false => { s' with specializations := s'.specializations.cons sub .nil }
+  | true => { s' with specializations := s'.specializations.replace sub sups }
+
+def Syntax.toState (s: Syntax): State :=
+  match s with 
+  | .leaf =>
+    .empty
+  | .withDeclaration d s =>
+    s.toState.withDecl d
+  | .withSpecialization sub sup s => 
+    s.toState.withSpecialization sub sup
+
+def st1 := s1.toState
+#eval st1
+
+end MWE6
